<?xml version="1.0" encoding="UTF-8"?>

<section xml:id="section-BLE">
    <title>Biconditionals, Logical Equivalence</title>

    <subsection>
        <title>Biconditional</title>
        <definition>
            <p>
                The <term>biconditional</term>, <m>P \leftrightarrow Q</m> is true if <m>P</m> and <m>Q</m> are either both true and both false, and is false if one of them is true and one is false.
            </p>
        </definition>

        <p>
            In other words, <m>P \leftrightarrow Q</m> is true if both statements share the same truth value.
        </p>
        <p>
            The truth table for a biconditional is given by,
        </p>
        <me>
            \begin{array}{c|c|c}
                P \amp Q \amp P \leftrightarrow Q  \\ \hline
                T \amp T \amp T \\ \hline
                T \amp F \amp F \\ \hline
                F \amp T \amp F \\ \hline
                F \amp F \amp T
            \end{array}
        </me>
        <p>
            With a biconditional, either both statements are true, or both are false. If one is true, then so is the other, and if one is false, then so is the other.
        </p>
        <p>
            Other ways to say <m>P \leftrightarrow Q</m> include <q><m>P</m> occurs <em>precisely when</em> <m>Q</m> occurs.</q>, <q>If <m>P</m>, then <m>Q</m>, and conversely.</q>, <q><m>P</m> is a necessary and sufficient condition for <m>Q</m>.</q>
        </p>
        <p>
            In English, some conditionals are implicitly biconditionals. In mathematics, we try to be more precise.
        </p>
    </subsection>

    <subsection>
        <title>Logical Equivalence</title>
        <p>
            If two statements have the same truth values in every case, then we say that <m>P</m> and <m>Q</m> are <term>logically equivalent</term>, and this is denoted by <m>P \equiv Q</m>. Roughly, this means that the two statements are <q>equal</q>, in the sense of logic.
        </p>
        <p>
            This notation allows us to describe some of the previous logical connectives in terms of more basic logical connectives. For example,
        </p>
        <ul>
            <li>For a biconditional, <m>P \leftrightarrow Q \equiv (P \rightarrow Q) \land (Q \rightarrow P)</m>. The truth table is given by,
                <me>
                    \begin{array}{c|c|c|c|c|c}
                        P \amp Q \amp P \leftrightarrow Q \amp P \rightarrow Q \amp Q \rightarrow P \amp (P \rightarrow Q) \land (Q \rightarrow P) \\ \hline
                        T \amp T \amp T \amp T \amp T \amp T \\ \hline
                        T \amp F \amp F \amp F \amp T \amp F \\ \hline
                        F \amp T \amp F \amp T \amp F \amp F \\ \hline
                        F \amp F \amp T \amp T \amp T \amp T
                    \end{array}
                </me>
            Notice that the column for <m>P \leftrightarrow Q</m> and for <m>(P \rightarrow Q) \land (Q \rightarrow P)</m> have the same truth value in every case.
            </li>
            <li>Previously, we saw that a conditional is logically equivalent to its contrapositive.</li>
            <li>The definition of conditional says that <m>P \rightarrow Q</m> is false if (and only if) <m>P</m> is true and <m>Q</m> is false. This means that,
            <me>
                \neg (P \rightarrow Q) \equiv P \land \neg Q
            </me></li>
            <li>Recall that the negation of a negation is equivalent to the original statement. In other words,
                <me>
                    \neg (\neg P) \equiv P
                </me>
            </li>
            <li>The converse of a condition is logically equivalent to the inverse. This can be seen by comparing the truth tables.</li>
            <li>The converse is not logically equivalent to the original conditional. Incorrectly assuming this this is called the <term>fallacy of the converse</term>.</li>
            <li>The inverse of a conditional is not logically equivalent to the conditional. Incorrectly assuming this is called <term>denying the antecedent</term>, or <term>fallacy of the inverse</term>.</li>
        </ul>
    </subsection>

    <subsection>
        <title>Order of Operations for Logical Operators</title>
    </subsection>

</section>
