<?xml version="1.0" encoding="UTF-8"?>

<section xml:id="section-ST">
    <title>Set Theorems</title>
    

    <subsection>
        <title>De Morgan's Laws</title>

        <p>
            The definitions of union and intersection rely on the logical <q>or</q> and <q>and</q>. This means to define the set complement of a union or intersection requires negating these <q>or</q> or <q>and</q> statements. First, by definition,
        </p>
        <md>
            <mrow>\overline{A \cup B} \amp = \set{x: x \notin A \cup B}</mrow>
            <mrow>\overline{A \cap B} \amp = \set{x: x \notin A \cap B}</mrow>
        </md>

        <theorem>
            <title>De Morgan's laws</title>
            <p>
                Let <m>A, B </m> be sets. Then,
            </p>
            <me>
                \overline{A \cap B} = \overline{A} \cup \overline{B} \qquad \text{and} \qquad \overline{A \cup B} = \overline{A} \cap \overline{B}
            </me>
            <p>
                In other words,
            </p>
            <ul>
                <li><m>x \notin A \cup B</m> if and only if <m>x \notin A</m> and <m>x \notin B</m>.</li>
                <li><m>x \notin A \cap B</m> if and only if <m>x \notin A</m> or <m>x \notin B</m></li>
            </ul>
        </theorem>

        <p>
            Again, recall De Morgan's laws,
        </p>
        <me>
            \neg (P \land Q) \equiv (\neg P) \lor (\neg Q) \amp\amp \text{and} \amp\amp \neg (P \lor Q) \equiv (\neg P) \land (\neg Q)
        </me>

        <proof>
            <p>
                First, consider <m>\overline{A \cup B}</m>.
            </p>
            <md>
                <mrow>x \in \overline{A \cup B} \equiv x \notin A \cup B \amp \equiv \neg (x \in A \cup B)</mrow>
                <mrow>\amp \equiv \neg (x \in A \lor x \in B)</mrow>
                <mrow>\amp \equiv \brac{\neg (x \in A) \land \neg (x \in B)} \amp\amp \text{by De Morgan's laws}</mrow>
                <mrow>\amp \equiv \brac{x \notin A \land x \notin B}</mrow>
                <mrow>\amp \equiv \brac{x \in \overline{A} \land x \in \overline{B}}</mrow>
                <mrow>\amp \equiv \brac{x \in \overline{A} \cap \overline{B}}</mrow>
            </md>
            <p>
                Similarly, for <m>\overline{A \cap B}</m>, the steps are similar, except replacing <q>and</q> with <q>or</q>,
            </p>
            <md>
                <mrow>x \in \overline{A \cap B} \equiv x \notin A \cap B \amp \equiv \neg (x \in A \cap B)</mrow>
                <mrow>\amp \equiv \neg (x \in A \land x \in B)</mrow>
                <mrow>\amp \equiv \brac{\neg (x \in A) \lor \neg (x \in B)} \amp\amp \text{by De Morgan's laws}</mrow>
                <mrow>\amp \equiv \brac{x \notin A \lor x \notin B}</mrow>
                <mrow>\amp \equiv \brac{x \in \overline{A} \lor x \in \overline{B}}</mrow>
                <mrow>\amp \equiv \brac{x \in \overline{A} \cup \overline{B}}</mrow>
            </md>
        </proof>
    </subsection>

    <subsection>
        <title>Distributive Property of Union and Intersection</title>
        <theorem>
            <p>
                Let <m>A, B, C</m> be sets. Then,
                <me>
                    A \cup (B \cap C) = (A \cup B) \cap (A \cup C) \qquad A \cap (B \cup C) = (A \cap B) \cup (A \cap C)
                </me>
            </p>
        </theorem>

        <proof>
            <p>
                First,
            </p>
            <md>
                <mrow>x \in A \cup (B \cap C) \amp \equiv x \in A \lor x \in B \cap C</mrow>
                <mrow>\amp \equiv x \in A \lor (x \in B \land x \in C)</mrow>
                <mrow>\amp \equiv \brac{x \in A \lor x \in B} \land \brac{x \in A \lor x \in C} \amp\amp \text{by distributive property of disjunction over conjunction}</mrow>
                <mrow>\amp \equiv \brac{x \in A \cup B} \land \brac{x \in A \cup C}</mrow>
                <mrow>\amp \equiv x \in (A \cup B) \cap (A \cup C)</mrow>
            </md>
            <p>
                Then, similarly,
            </p>
            <md>
                <mrow>x \in A \cap (B \cap C) \amp \equiv x \in A \land x \in B \cup C</mrow>
                <mrow>\amp \equiv x \in A \land (x \in B \lor x \in C)</mrow>
                <mrow>\amp \equiv \brac{x \in A \land x \in B} \lor \brac{x \in A \land x \in C} \amp\amp \text{by distributive property of disjunction over conjunction}</mrow>
                <mrow>\amp \equiv \brac{x \in A \cap B} \lor \brac{x \in A \cap C}</mrow>
                <mrow>\amp \equiv x \in (A \cap B) \cup (A \cap C)</mrow>
            </md>
        </proof>


    </subsection>
</section>
